src/riscv/Examples/smt/testInductive.smt
@@ -22,9 +22,52 @@
   (ThreadEvent (Tid_of_ThreadEvent ThreadId) (Iid_of_ThreadEvent EventId))
 )))
 
+(define-fun NextEvent ((e Event)) Event
+  (match e (
+    ((InitEvent x) e)
+    ((ThreadEvent t i) (ThreadEvent t (+ i 1))))))
+
 (declare-datatypes () ((InstructionI
-  (Lb (rd_of_Lb Z) (rs1_of_Lb Z) (oimm12_of_Lb Z))
-  (Sb (rs1_of_Sb Z) (rs2_of_Sb Z) (simm12_of_Sb Z))
+   (Lb (rd_Lb Z) (rs1_Lb Z) (oimm12_Lb Z))
+   (Lh (rd_Lh Z) (rs1_Lh Z) (oimm12_Lh Z))
+   (Lw (rd_Lw Z) (rs1_Lw Z) (oimm12_Lw Z))
+   (Lbu (rd_Lbu Z) (rs1_Lbu Z) (oimm12_Lbu Z))
+   (Lhu (rd_Lhu Z) (rs1_Lhu Z) (oimm12_Lhu Z))
+   (Fence (pred_Fence Z) (succ_Fence Z))
+   Fence_i
+   (Addi (rd_Addi Z) (rs1_Addi Z) (imm12_Addi Z))
+   (Slli (rd_Slli Z) (rs1_Slli Z) (shamt6_Slli Z))
+   (Slti (rd_Slti Z) (rs1_Slti Z) (imm12_Slti Z))
+   (Sltiu (rd_Sltiu Z) (rs1_Sltiu Z) (imm12_Sltiu Z))
+   (Xori (rd_Xori Z) (rs1_Xori Z) (imm12_Xori Z))
+   (Ori (rd_Ori Z) (rs1_Ori Z) (imm12_Ori Z))
+   (Andi (rd_Andi Z) (rs1_Andi Z) (imm12_Andi Z))
+   (Srli (rd_Srli Z) (rs1_Srli Z) (shamt6_Srli Z))
+   (Srai (rd_Srai Z) (rs1_Srai Z) (shamt6_Srai Z))
+   (Auipc (rd_Auipc Z) (oimm20_Auipc Z))
+   (Sb (rs1_Sb Z) (rs2_Sb Z) (simm12_Sb Z))
+   (Sh (rs1_Sh Z) (rs2_Sh Z) (simm12_Sh Z))
+   (Sw (rs1_Sw Z) (rs2_Sw Z) (simm12_Sw Z))
+   (Add (rd_Add Z) (rs1_Add Z) (rs2_Add Z))
+   (Sub (rd_Sub Z) (rs1_Sub Z) (rs2_Sub Z))
+   (Sll (rd_Sll Z) (rs1_Sll Z) (rs2_Sll Z))
+   (Slt (rd_Slt Z) (rs1_Slt Z) (rs2_Slt Z))
+   (Sltu (rd_Sltu Z) (rs1_Sltu Z) (rs2_Sltu Z))
+   (Xor (rd_Xor Z) (rs1_Xor Z) (rs2_Xor Z))
+   (Srl (rd_Srl Z) (rs1_Srl Z) (rs2_Srl Z))
+   (Sra (rd_Sra Z) (rs1_Sra Z) (rs2_Sra Z))
+   (Or (rd_Or Z) (rs1_Or Z) (rs2_Or Z))
+   (And (rd_And Z) (rs1_And Z) (rs2_And Z))
+   (Lui (rd_Lui Z) (imm20_Lui Z))
+   (Beq (rs1_Beq Z) (rs2_Beq Z) (sbimm12_Beq Z))
+   (Bne (rs1_Bne Z) (rs2_Bne Z) (sbimm12_Bne Z))
+   (Blt (rs1_Blt Z) (rs2_Blt Z) (sbimm12_Blt Z))
+   (Bge (rs1_Bge Z) (rs2_Bge Z) (sbimm12_Bge Z))
+   (Bltu (rs1_Bltu Z) (rs2_Bltu Z) (sbimm12_Bltu Z))
+   (Bgeu (rs1_Bgeu Z) (rs2_Bgeu Z) (sbimm12_Bgeu Z))
+   (Jalr (rd_Jalr Z) (rs1_Jalr Z) (oimm12_Jalr Z))
+   (Jal (rd_Jal Z) (jimm20_Jal Z))
+   InvalidI
 )))
 
 ; that's just the register name, needs to be between 0 and 32, value will be of type word
@@ -36,66 +79,64 @@
   (Regs Registers)
   (Pc word)
   (NextPc word)
-  (Prog (Array Int InstructionI))
+  (Prog (Array word InstructionI))
   (CurrentEvent Event)
   (Deps (Array Register (set Event)))
 ))))
+
+(define-fun withRegs         ((x Registers                   ) (s ThreadState)) ThreadState (mkThreadState x        (Pc s) (NextPc s) (Prog s) (CurrentEvent s) (Deps s)))
+(define-fun withPc           ((x word                        ) (s ThreadState)) ThreadState (mkThreadState (Regs s) x      (NextPc s) (Prog s) (CurrentEvent s) (Deps s)))
+(define-fun withNextPc       ((x word                        ) (s ThreadState)) ThreadState (mkThreadState (Regs s) (Pc s) x          (Prog s) (CurrentEvent s) (Deps s)))
+(define-fun withProg         ((x (Array word InstructionI)    ) (s ThreadState)) ThreadState (mkThreadState (Regs s) (Pc s) (NextPc s) x        (CurrentEvent s) (Deps s)))
+(define-fun withCurrentEvent ((x Event                       ) (s ThreadState)) ThreadState (mkThreadState (Regs s) (Pc s) (NextPc s) (Prog s) x                (Deps s)))
+(define-fun withDeps         ((x (Array Register (set Event))) (s ThreadState)) ThreadState (mkThreadState (Regs s) (Pc s) (NextPc s) (Prog s) (CurrentEvent s) x       ))
 
 (declare-datatypes () ((Label
   (ReadLabel (LabelReadLoc word))
   (WriteLabel (LabelWriteLoc word) (LabelVal w8))
   FenceLabel
-  ErrorLabel)))
+  ErrorLabel
+  AbsentLabel)))
+
+(declare-datatypes () ((EventTyp ReadEvent WriteEvent FenceEvent ErrorEvent AbsentEvent)))
+
+(define-fun LabelTyp ((l Label)) EventTyp
+  (match l (
+    ((ReadLabel _) ReadEvent)
+    ((WriteLabel _ _) WriteEvent)
+    (FenceLabel FenceEvent)
+    (ErrorLabel ErrorEvent)
+    (AbsentLabel AbsentEvent))))
 
 (declare-datatypes () ((Graph (mkGraph
-  (Lab (Array Event (option Label)))
+  (Lab (Array Event Label))
   (Rf (Array Event Event))
   (Addr (Array Event (set Event)))
   (Data (Array Event (set Event)))
   (Ctrl (Array Event (set Event)))
 ))))
 
-(define-fun Loc00 ((G Graph) (e Event)) (option Label)
-  (match (select (Lab G) e) (
-    ((Some l) (match (Some l) (
-                 ((Some ll) (Some ll))
-                 (None None))))
-    (None None))))
+(define-fun Typ ((G Graph) (e Event)) EventTyp (LabelTyp (select (Lab G) e)))
 
-(define-fun LocOfLabel ((l Label)) (option word)
-  (match l (
-    ((ReadLabel x) (Some x))
-    ((WriteLabel x v) (Some x))
-    (FenceLabel (as None (option word)))
-    (ErrorLabel (as None (option word))))))
-
-(define-fun Loc001 ((G Graph) (e Event)) (option word)
-  (match (select (Lab G) e) (
-    ((Some theL) (LocOfLabel theL))
-    (None None))))
+(declare-const G0 Graph)
+(declare-const e0 Event)
+(assert (= (select (Lab G0) e0) AbsentLabel))
 
 (define-fun Loc ((G Graph) (e Event)) (option word)
   (match (select (Lab G) e) (
-    ((Some ll) (match ll (
-                ((ReadLabel x) (Some x))
-                ((WriteLabel x v) (Some x))
-                (FenceLabel None)
-                (ErrorLabel None))))
-    (None None))))
+    ((ReadLabel x) (Some x))
+    ((WriteLabel x v) (Some x))
+    (FenceLabel (as None (option word)))
+    (ErrorLabel (as None (option word)))
+    (AbsentLabel (as None (option word))))))
 
-(declare-fun Val ((G Graph) (e Event)) (option w8)
+(define-fun Val ((G Graph) (e Event)) w8
   (match (select (Lab G) e) (
-    ((Some l) (match l (
-                ((ReadLabel x) None)
-                ((WriteLabel x v) (Some v))
-                (FenceLabel None)
-                (ErrorLabel None))))
-    (None None))))
-
-(define-fun executeIsmall ((inst InstructionI) (s1 ThreadState) (s2 ThreadState)) bool
-  (match inst (
-    ((Lb rd rs1 oimm12) (= s1 s2))
-    ((Sb rs1 rs2 simm12) (not (= s1 s2))))))
+    ((ReadLabel x) #x00)
+    ((WriteLabel x v) v)
+    (FenceLabel #x00)
+    (ErrorLabel #x00)
+    (AbsentLabel #x00))))
 
 (declare-const nn Int)
 (assert (exists ((a Int)) (and (< 2 a) (= nn (* a a)))))
@@ -104,7 +145,6 @@
 (declare-const i2 InstructionI)
 (declare-const s ThreadState)
 (assert (not (= i1 i2)))
-(assert (executeIsmall i1 s s))
 
 (define-fun getReg ((regs Registers) (reg Register)) word
   (ite (= reg 0) ((_ int2bv 32) 0) (select regs reg)))
@@ -112,154 +152,417 @@
 (define-fun setReg ((regs Registers) (reg Register) (v word)) Registers
   (ite (= reg 0) regs (store regs reg v)))
 
-(define-fun executeI ((G Graph) (inst InstructionI) (s1 ThreadState) (s2 ThreadState)) bool
-  (match inst (   ( (Lb rd rs1
-oimm12) (exists ( (_ unit)
-         ) (and (= (select (Lab G) (CurrentEvent s1))
-                 (Some (ReadLabel (bvadd (getReg (Regs s1) rs1) ((_ int2bv 32) oimm12)))))
-            (exists ( (v0 w8)
-             ) (and (= (Val G (select (Rf G) (CurrentEvent s1))) (Some v0))
-                (and (=
-                      (withRegs
-                         (setReg (Regs s1) rd ((_ int2bv 32) (signExtend 8 (LittleEndian.combine 1 v0))))
-                         (withCurrentEvent (NextEvent (CurrentEvent s1)) s1)) s2)
-                 (= tt tt)))))))   ( (Lh _ _
-_) (exists ( (_ unit)) (and (= (select (Lab G) (CurrentEvent s1)) (Some ErrorLabel)) (= s1 s2))))   ( (Lw _ _
-_) (exists ( (_ unit)) (and (= (select (Lab G) (CurrentEvent s1)) (Some ErrorLabel)) (= s1 s2))))   ( (Lbu rd
-rs1
-oimm12) (exists ( (_ unit)
-         ) (and (= (select (Lab G) (CurrentEvent s1))
-                 (Some (ReadLabel (bvadd (getReg (Regs s1) rs1) ((_ int2bv 32) oimm12)))))
-            (exists ( (v0 w8)
-             ) (and (= (Val G (select (Rf G) (CurrentEvent s1))) (Some v0))
-                (and (=
-                      (withRegs (setReg (Regs s1) rd ((_ int2bv 32) (LittleEndian.combine 1 v0)))
-                         (withCurrentEvent (NextEvent (CurrentEvent s1)) s1)) s2)
-                 (= tt tt)))))))   ( (Lhu _ _
-_) (exists ( (_ unit)) (and (= (select (Lab G) (CurrentEvent s1)) (Some ErrorLabel)) (= s1 s2))))   ( (Fence _
-_) (and (= s1 s2) (= tt tt)))   ( (Fence_i ) (and (= s1 s2) (= tt tt)))   ( (Addi rd rs1
-imm12) (and (= (withRegs (setReg (Regs s1) rd (bvadd (getReg (Regs s1) rs1) ((_ int2bv 32) imm12))) s1) s2)
-        (= tt tt)))   ( (Slli rd rs1
-shamt6) (and (= (withRegs (setReg (Regs s1) rd (word.slu (getReg (Regs s1) rs1) ((_ int2bv 32) shamt6))) s1)
-              s2) (= tt tt)))   ( (Slti rd rs1
-imm12) (and (=
-             (withRegs
-                (setReg (Regs s1) rd
-                   (ite (bvlts (getReg (Regs s1) rs1) ((_ int2bv 32) imm12)) ((_ int2bv 32) 1)
-                    ((_ int2bv 32) 0))) s1) s2) (= tt tt)))   ( (Sltiu rd rs1
-imm12) (and (=
-             (withRegs
-                (setReg (Regs s1) rd
-                   (ite (bvltu (getReg (Regs s1) rs1) ((_ int2bv 32) imm12)) ((_ int2bv 32) 1)
-                    ((_ int2bv 32) 0))) s1) s2) (= tt tt)))   ( (Xori rd rs1
-imm12) (and (= (withRegs (setReg (Regs s1) rd (bvxor (getReg (Regs s1) rs1) ((_ int2bv 32) imm12))) s1) s2)
-        (= tt tt)))   ( (Ori rd rs1
-imm12) (and (= (withRegs (setReg (Regs s1) rd (word.or (getReg (Regs s1) rs1) ((_ int2bv 32) imm12))) s1) s2)
-        (= tt tt)))   ( (Andi rd rs1
-imm12) (and (= (withRegs (setReg (Regs s1) rd (bvand (getReg (Regs s1) rs1) ((_ int2bv 32) imm12))) s1) s2)
-        (= tt tt)))   ( (Srli rd rs1
-shamt6) (and (= (withRegs (setReg (Regs s1) rd (word.sru (getReg (Regs s1) rs1) ((_ int2bv 32) shamt6))) s1)
-              s2) (= tt tt)))   ( (Srai rd rs1
-shamt6) (and (= (withRegs (setReg (Regs s1) rd (word.srs (getReg (Regs s1) rs1) ((_ int2bv 32) shamt6))) s1)
-              s2) (= tt tt)))   ( (Auipc rd
-oimm20) (and (= (withRegs (setReg (Regs s1) rd (bvadd ((_ int2bv 32) oimm20) (Pc s1))) s1) s2) (= tt tt)))
-( (Sb rs1 rs2
-simm12) (exists ( (_ unit)
-         ) (and (= (select (Lab G) (CurrentEvent s1))
-                 (Some
-                    (WriteLabel (bvadd (getReg (Regs s1) rs1) ((_ int2bv 32) simm12))
-                       (LittleEndian.split 1 (word.unsigned (getReg (Regs s1) rs2))))))
-            (and (= (withCurrentEvent (NextEvent (CurrentEvent s1)) s1) s2) (= tt tt)))))   ( (Sh _ _
-_) (exists ( (_ unit)) (and (= (select (Lab G) (CurrentEvent s1)) (Some ErrorLabel)) (= s1 s2))))   ( (Sw _ _
-_) (exists ( (_ unit)) (and (= (select (Lab G) (CurrentEvent s1)) (Some ErrorLabel)) (= s1 s2))))   ( (Add rd
-rs1
-rs2) (and (= (withRegs (setReg (Regs s1) rd (bvadd (getReg (Regs s1) rs1) (getReg (Regs s1) rs2))) s1) s2)
-      (= tt tt)))   ( (Sub rd rs1
-rs2) (and (= (withRegs (setReg (Regs s1) rd (word.sub (getReg (Regs s1) rs1) (getReg (Regs s1) rs2))) s1) s2)
-      (= tt tt)))   ( (Sll rd rs1
-rs2) (and (=
-           (withRegs
-              (setReg (Regs s1) rd
-                 (word.slu (getReg (Regs s1) rs1)
-                    ((_ int2bv 32) (word.unsigned (getReg (Regs s1) rs2) mod 32)))) s1) s2)
-      (= tt tt)))   ( (Slt rd rs1
-rs2) (and (=
-           (withRegs
-              (setReg (Regs s1) rd
-                 (ite (bvlts (getReg (Regs s1) rs1) (getReg (Regs s1) rs2)) ((_ int2bv 32) 1)
-                  ((_ int2bv 32) 0))) s1) s2) (= tt tt)))   ( (Sltu rd rs1
-rs2) (and (=
-           (withRegs
-              (setReg (Regs s1) rd
-                 (ite (bvltu (getReg (Regs s1) rs1) (getReg (Regs s1) rs2)) ((_ int2bv 32) 1)
-                  ((_ int2bv 32) 0))) s1) s2) (= tt tt)))   ( (Xor rd rs1
-rs2) (and (= (withRegs (setReg (Regs s1) rd (bvxor (getReg (Regs s1) rs1) (getReg (Regs s1) rs2))) s1) s2)
-      (= tt tt)))   ( (Srl rd rs1
-rs2) (and (=
-           (withRegs
-              (setReg (Regs s1) rd
-                 (word.sru (getReg (Regs s1) rs1)
-                    ((_ int2bv 32) (word.unsigned (getReg (Regs s1) rs2) mod 32)))) s1) s2)
-      (= tt tt)))   ( (Sra rd rs1
-rs2) (and (=
-           (withRegs
-              (setReg (Regs s1) rd
-                 (word.srs (getReg (Regs s1) rs1)
-                    ((_ int2bv 32) (word.unsigned (getReg (Regs s1) rs2) mod 32)))) s1) s2)
-      (= tt tt)))   ( (Or rd rs1
-rs2) (and (= (withRegs (setReg (Regs s1) rd (word.or (getReg (Regs s1) rs1) (getReg (Regs s1) rs2))) s1) s2)
-      (= tt tt)))   ( (And rd rs1
-rs2) (and (= (withRegs (setReg (Regs s1) rd (bvand (getReg (Regs s1) rs1) (getReg (Regs s1) rs2))) s1) s2)
-      (= tt tt)))   ( (Lui rd
-imm20) (and (= (withRegs (setReg (Regs s1) rd ((_ int2bv 32) imm20)) s1) s2) (= tt tt)))   ( (Beq rs1 rs2
-sbimm12) (ite (= (getReg (Regs s1) rs1) (getReg (Regs s1) rs2))
-          (ite (negb (= (bvurem (bvadd (Pc s1) ((_ int2bv 32) sbimm12)) ((_ int2bv 32) 4)) ((_ int2bv 32) 0)))
-           (exists ( (_ unit)) (and (= (select (Lab G) (CurrentEvent s1)) (Some ErrorLabel)) (= s1 s2)))
-           (and (= (withNextPc (bvadd (Pc s1) ((_ int2bv 32) sbimm12)) s1) s2) (= tt tt)))
-          (and (= s1 s2) (= tt tt))))   ( (Bne rs1 rs2
-sbimm12) (ite (negb (= (getReg (Regs s1) rs1) (getReg (Regs s1) rs2)))
-          (ite (negb (= (bvurem (bvadd (Pc s1) ((_ int2bv 32) sbimm12)) ((_ int2bv 32) 4)) ((_ int2bv 32) 0)))
-           (exists ( (_ unit)) (and (= (select (Lab G) (CurrentEvent s1)) (Some ErrorLabel)) (= s1 s2)))
-           (and (= (withNextPc (bvadd (Pc s1) ((_ int2bv 32) sbimm12)) s1) s2) (= tt tt)))
-          (and (= s1 s2) (= tt tt))))   ( (Blt rs1 rs2
-sbimm12) (ite (bvlts (getReg (Regs s1) rs1) (getReg (Regs s1) rs2))
-          (ite (negb (= (bvurem (bvadd (Pc s1) ((_ int2bv 32) sbimm12)) ((_ int2bv 32) 4)) ((_ int2bv 32) 0)))
-           (exists ( (_ unit)) (and (= (select (Lab G) (CurrentEvent s1)) (Some ErrorLabel)) (= s1 s2)))
-           (and (= (withNextPc (bvadd (Pc s1) ((_ int2bv 32) sbimm12)) s1) s2) (= tt tt)))
-          (and (= s1 s2) (= tt tt))))   ( (Bge rs1 rs2
-sbimm12) (ite (negb (bvlts (getReg (Regs s1) rs1) (getReg (Regs s1) rs2)))
-          (ite (negb (= (bvurem (bvadd (Pc s1) ((_ int2bv 32) sbimm12)) ((_ int2bv 32) 4)) ((_ int2bv 32) 0)))
-           (exists ( (_ unit)) (and (= (select (Lab G) (CurrentEvent s1)) (Some ErrorLabel)) (= s1 s2)))
-           (and (= (withNextPc (bvadd (Pc s1) ((_ int2bv 32) sbimm12)) s1) s2) (= tt tt)))
-          (and (= s1 s2) (= tt tt))))   ( (Bltu rs1 rs2
-sbimm12) (ite (bvltu (getReg (Regs s1) rs1) (getReg (Regs s1) rs2))
-          (ite (negb (= (bvurem (bvadd (Pc s1) ((_ int2bv 32) sbimm12)) ((_ int2bv 32) 4)) ((_ int2bv 32) 0)))
-           (exists ( (_ unit)) (and (= (select (Lab G) (CurrentEvent s1)) (Some ErrorLabel)) (= s1 s2)))
-           (and (= (withNextPc (bvadd (Pc s1) ((_ int2bv 32) sbimm12)) s1) s2) (= tt tt)))
-          (and (= s1 s2) (= tt tt))))   ( (Bgeu rs1 rs2
-sbimm12) (ite (negb (bvltu (getReg (Regs s1) rs1) (getReg (Regs s1) rs2)))
-          (ite (negb (= (bvurem (bvadd (Pc s1) ((_ int2bv 32) sbimm12)) ((_ int2bv 32) 4)) ((_ int2bv 32) 0)))
-           (exists ( (_ unit)) (and (= (select (Lab G) (CurrentEvent s1)) (Some ErrorLabel)) (= s1 s2)))
-           (and (= (withNextPc (bvadd (Pc s1) ((_ int2bv 32) sbimm12)) s1) s2) (= tt tt)))
-          (and (= s1 s2) (= tt tt))))   ( (Jalr rd rs1
-oimm12) (ite (negb
-                (=
-                 (bvurem (bvand (bvadd (getReg (Regs s1) rs1) ((_ int2bv 32) oimm12))
-                          (bvxor ((_ int2bv 32) 1) ((_ int2bv 32) 4294967295))) ((_ int2bv 32) 4))
-                 ((_ int2bv 32) 0)))
-         (exists ( (_ unit)) (and (= (select (Lab G) (CurrentEvent s1)) (Some ErrorLabel)) (= s1 s2)))
-         (and (=
-               (withNextPc
-                  (bvand (bvadd (getReg (Regs s1) rs1) ((_ int2bv 32) oimm12))
-                   (bvxor ((_ int2bv 32) 1) ((_ int2bv 32) 4294967295)))
-                  (withRegs (setReg (Regs s1) rd (bvadd (Pc s1) ((_ int2bv 32) 4))) s1)) s2)
-          (= tt tt))))   ( (Jal rd
-jimm20) (ite (negb (= (bvurem (bvadd (Pc s1) ((_ int2bv 32) jimm20)) ((_ int2bv 32) 4)) ((_ int2bv 32) 0)))
-         (exists ( (_ unit)) (and (= (select (Lab G) (CurrentEvent s1)) (Some ErrorLabel)) (= s1 s2)))
-         (and (=
-               (withNextPc (bvadd (Pc s1) ((_ int2bv 32) jimm20))
-                  (withRegs (setReg (Regs s1) rd (bvadd (Pc s1) ((_ int2bv 32) 4))) s1)) s2)
-          (= tt tt))))   ( (InvalidI ) (and (= s1 s2) (= tt tt))))))
+(define-const emptyEvents (set Event) ((as const (set Event)) false))
+(define-const emptyDeps (Array Register (set Event)) ((as const (Array Register (set Event))) emptyEvents))
 
+(define-fun getDeps ((D (Array Register (set Event))) (r Register)) (set Event)
+  (ite (= r 0) emptyEvents (select D r)))
+
+(define-fun setDeps ((D (Array Register (set Event))) (r Register) (s (set Event))) (Array Register (set Event))
+  (ite (= r 0) D (store D r s)))
+
+(define-const minusone Int (- 1))
+
+(define-fun run1 ((G Graph) (s1 ThreadState) (s2 ThreadState)) bool
+(match (select (Prog s1) (Pc s1)) (
+((Lb rd rs1 oimm12) (and (and (= (select (Addr G) (CurrentEvent s1)) (getDeps (Deps s1) rs1))
+                          (and (= (select (Data G) (CurrentEvent s1)) emptyEvents)
+                           (= (select (Ctrl G) (CurrentEvent s1)) (getDeps (Deps s1) minusone))))
+                     (and (and (= (select (Lab G) (CurrentEvent s1))
+                                (ReadLabel (bvadd (getReg (Regs s1) rs1) ((_ int2bv 32) oimm12))))
+                           (= (Typ G (select (Rf G) (CurrentEvent s1))) WriteEvent))
+                      (and (=
+                            (withPc (NextPc s1)
+                               (withNextPc (bvadd (NextPc s1) ((_ int2bv 32) 4))
+                                  (withDeps (Deps s1)
+                                     (withRegs
+                                        (setReg (Regs s1) rd
+                                           ((_ sign_extend 24) (Val G (select (Rf G) (CurrentEvent s1)))))
+                                        (withCurrentEvent (NextEvent (CurrentEvent s1)) s1))))) s2)
+                       (= tt tt)))))
+((Lh _ _ _) (and (= (select (Lab G) (CurrentEvent s1)) ErrorLabel) (= s1 s2)))
+((Lw _ _ _) (and (= (select (Lab G) (CurrentEvent s1)) ErrorLabel) (= s1 s2)))
+((Lbu rd rs1 oimm12) (and (and (= (select (Lab G) (CurrentEvent s1))
+                                (ReadLabel (bvadd (getReg (Regs s1) rs1) ((_ int2bv 32) oimm12))))
+                           (= (Typ G (select (Rf G) (CurrentEvent s1))) WriteEvent))
+                      (and (=
+                            (withPc (NextPc s1)
+                               (withNextPc (bvadd (NextPc s1) ((_ int2bv 32) 4))
+                                  (withDeps (Deps s1)
+                                     (withRegs
+                                        (setReg (Regs s1) rd
+                                           ((_ zero_extend 24) (Val G (select (Rf G) (CurrentEvent s1)))))
+                                        (withCurrentEvent (NextEvent (CurrentEvent s1)) s1))))) s2)
+                       (= tt tt))))
+((Lhu _ _ _) (and (= (select (Lab G) (CurrentEvent s1)) ErrorLabel) (= s1 s2)))
+((Fence _ _) (and (=
+                   (withPc (NextPc s1)
+                      (withNextPc (bvadd (NextPc s1) ((_ int2bv 32) 4)) (withDeps (Deps s1) s1))) s2)
+              (= tt tt)))
+((Fence_i) (and (=
+                 (withPc (NextPc s1)
+                    (withNextPc (bvadd (NextPc s1) ((_ int2bv 32) 4)) (withDeps (Deps s1) s1))) s2)
+            (= tt tt)))
+((Addi rd rs1 imm12) (and (=
+                           (withPc (NextPc s1)
+                              (withNextPc (bvadd (NextPc s1) ((_ int2bv 32) 4))
+                                 (withDeps (setDeps (Deps s1) rd (getDeps (Deps s1) rs1))
+                                    (withRegs
+                                       (setReg (Regs s1) rd
+                                          (bvadd (getReg (Regs s1) rs1) ((_ int2bv 32) imm12))) s1)))) s2)
+                      (= tt tt)))
+((Slli rd rs1 shamt6) (and (=
+                            (withPc (NextPc s1)
+                               (withNextPc (bvadd (NextPc s1) ((_ int2bv 32) 4))
+                                  (withDeps (setDeps (Deps s1) rd (getDeps (Deps s1) rs1))
+                                     (withRegs
+                                        (setReg (Regs s1) rd
+                                           (bvshl (getReg (Regs s1) rs1) ((_ int2bv 32) shamt6))) s1)))) s2)
+                       (= tt tt)))
+((Slti rd rs1 imm12) (and (=
+                           (withPc (NextPc s1)
+                              (withNextPc (bvadd (NextPc s1) ((_ int2bv 32) 4))
+                                 (withDeps (setDeps (Deps s1) rd (getDeps (Deps s1) rs1))
+                                    (withRegs
+                                       (setReg (Regs s1) rd
+                                          (ite (bvslt (getReg (Regs s1) rs1) ((_ int2bv 32) imm12))
+                                           ((_ int2bv 32) 1) ((_ int2bv 32) 0))) s1)))) s2)
+                      (= tt tt)))
+((Sltiu rd rs1 imm12) (and (=
+                            (withPc (NextPc s1)
+                               (withNextPc (bvadd (NextPc s1) ((_ int2bv 32) 4))
+                                  (withDeps (setDeps (Deps s1) rd (getDeps (Deps s1) rs1))
+                                     (withRegs
+                                        (setReg (Regs s1) rd
+                                           (ite (bvult (getReg (Regs s1) rs1) ((_ int2bv 32) imm12))
+                                            ((_ int2bv 32) 1) ((_ int2bv 32) 0))) s1)))) s2)
+                       (= tt tt)))
+((Xori rd rs1 imm12) (and (=
+                           (withPc (NextPc s1)
+                              (withNextPc (bvadd (NextPc s1) ((_ int2bv 32) 4))
+                                 (withDeps (setDeps (Deps s1) rd (getDeps (Deps s1) rs1))
+                                    (withRegs
+                                       (setReg (Regs s1) rd
+                                          (bvxor (getReg (Regs s1) rs1) ((_ int2bv 32) imm12))) s1)))) s2)
+                      (= tt tt)))
+((Ori rd rs1 imm12) (and (=
+                          (withPc (NextPc s1)
+                             (withNextPc (bvadd (NextPc s1) ((_ int2bv 32) 4))
+                                (withDeps (setDeps (Deps s1) rd (getDeps (Deps s1) rs1))
+                                   (withRegs
+                                      (setReg (Regs s1) rd (bvor (getReg (Regs s1) rs1) ((_ int2bv 32) imm12)))
+                                      s1)))) s2) (= tt tt)))
+((Andi rd rs1 imm12) (and (=
+                           (withPc (NextPc s1)
+                              (withNextPc (bvadd (NextPc s1) ((_ int2bv 32) 4))
+                                 (withDeps (setDeps (Deps s1) rd (getDeps (Deps s1) rs1))
+                                    (withRegs
+                                       (setReg (Regs s1) rd
+                                          (bvand (getReg (Regs s1) rs1) ((_ int2bv 32) imm12))) s1)))) s2)
+                      (= tt tt)))
+((Srli rd rs1 shamt6) (and (=
+                            (withPc (NextPc s1)
+                               (withNextPc (bvadd (NextPc s1) ((_ int2bv 32) 4))
+                                  (withDeps (setDeps (Deps s1) rd (getDeps (Deps s1) rs1))
+                                     (withRegs
+                                        (setReg (Regs s1) rd
+                                           (bvlshr (getReg (Regs s1) rs1) ((_ int2bv 32) shamt6))) s1)))) s2)
+                       (= tt tt)))
+((Srai rd rs1 shamt6) (and (=
+                            (withPc (NextPc s1)
+                               (withNextPc (bvadd (NextPc s1) ((_ int2bv 32) 4))
+                                  (withDeps (setDeps (Deps s1) rd (getDeps (Deps s1) rs1))
+                                     (withRegs
+                                        (setReg (Regs s1) rd
+                                           (bvashr (getReg (Regs s1) rs1) ((_ int2bv 32) shamt6))) s1)))) s2)
+                       (= tt tt)))
+((Auipc rd oimm20) (and (=
+                         (withPc (NextPc s1)
+                            (withNextPc (bvadd (NextPc s1) ((_ int2bv 32) 4))
+                               (withDeps (setDeps (Deps s1) rd (getDeps (Deps s1) minusone))
+                                  (withRegs (setReg (Regs s1) rd (bvadd ((_ int2bv 32) oimm20) (Pc s1))) s1))))
+                         s2) (= tt tt)))
+((Sb rs1 rs2 simm12) (and (and (= (select (Addr G) (CurrentEvent s1)) (getDeps (Deps s1) rs1))
+                           (and (= (select (Data G) (CurrentEvent s1)) (getDeps (Deps s1) rs2))
+                            (= (select (Ctrl G) (CurrentEvent s1)) (getDeps (Deps s1) minusone))))
+                      (and (= (select (Lab G) (CurrentEvent s1))
+                            (WriteLabel (bvadd (getReg (Regs s1) rs1) ((_ int2bv 32) simm12))
+                               ((_ extract 7 0) (getReg (Regs s1) rs2))))
+                       (and (=
+                             (withPc (NextPc s1)
+                                (withNextPc (bvadd (NextPc s1) ((_ int2bv 32) 4))
+                                   (withDeps (Deps s1) (withCurrentEvent (NextEvent (CurrentEvent s1)) s1))))
+                             s2) (= tt tt)))))
+((Sh _ _ _) (and (= (select (Lab G) (CurrentEvent s1)) ErrorLabel) (= s1 s2)))
+((Sw _ _ _) (and (= (select (Lab G) (CurrentEvent s1)) ErrorLabel) (= s1 s2)))
+((Add rd rs1 rs2) (and (=
+                        (withPc (NextPc s1)
+                           (withNextPc (bvadd (NextPc s1) ((_ int2bv 32) 4))
+                              (withDeps
+                                 (setDeps (Deps s1) rd (union (getDeps (Deps s1) rs1) (getDeps (Deps s1) rs2)))
+                                 (withRegs
+                                    (setReg (Regs s1) rd (bvadd (getReg (Regs s1) rs1) (getReg (Regs s1) rs2)))
+                                    s1)))) s2) (= tt tt)))
+((Sub rd rs1 rs2) (and (=
+                        (withPc (NextPc s1)
+                           (withNextPc (bvadd (NextPc s1) ((_ int2bv 32) 4))
+                              (withDeps
+                                 (setDeps (Deps s1) rd (union (getDeps (Deps s1) rs1) (getDeps (Deps s1) rs2)))
+                                 (withRegs
+                                    (setReg (Regs s1) rd (bvsub (getReg (Regs s1) rs1) (getReg (Regs s1) rs2)))
+                                    s1)))) s2) (= tt tt)))
+((Sll rd rs1 rs2) (and (=
+                        (withPc (NextPc s1)
+                           (withNextPc (bvadd (NextPc s1) ((_ int2bv 32) 4))
+                              (withDeps
+                                 (setDeps (Deps s1) rd (union (getDeps (Deps s1) rs1) (getDeps (Deps s1) rs2)))
+                                 (withRegs
+                                    (setReg (Regs s1) rd
+                                       (bvshl (getReg (Regs s1) rs1)
+                                        ((_ int2bv 32) (mod ((_ bv2nat 32) (getReg (Regs s1) rs2)) 32)))) s1))))
+                        s2) (= tt tt)))
+((Slt rd rs1 rs2) (and (=
+                        (withPc (NextPc s1)
+                           (withNextPc (bvadd (NextPc s1) ((_ int2bv 32) 4))
+                              (withDeps
+                                 (setDeps (Deps s1) rd (union (getDeps (Deps s1) rs1) (getDeps (Deps s1) rs2)))
+                                 (withRegs
+                                    (setReg (Regs s1) rd
+                                       (ite (bvslt (getReg (Regs s1) rs1) (getReg (Regs s1) rs2))
+                                        ((_ int2bv 32) 1) ((_ int2bv 32) 0))) s1)))) s2)
+                   (= tt tt)))
+((Sltu rd rs1 rs2) (and (=
+                         (withPc (NextPc s1)
+                            (withNextPc (bvadd (NextPc s1) ((_ int2bv 32) 4))
+                               (withDeps
+                                  (setDeps (Deps s1) rd
+                                     (union (getDeps (Deps s1) rs1) (getDeps (Deps s1) rs2)))
+                                  (withRegs
+                                     (setReg (Regs s1) rd
+                                        (ite (bvult (getReg (Regs s1) rs1) (getReg (Regs s1) rs2))
+                                         ((_ int2bv 32) 1) ((_ int2bv 32) 0))) s1)))) s2)
+                    (= tt tt)))
+((Xor rd rs1 rs2) (and (=
+                        (withPc (NextPc s1)
+                           (withNextPc (bvadd (NextPc s1) ((_ int2bv 32) 4))
+                              (withDeps
+                                 (setDeps (Deps s1) rd (union (getDeps (Deps s1) rs1) (getDeps (Deps s1) rs2)))
+                                 (withRegs
+                                    (setReg (Regs s1) rd (bvxor (getReg (Regs s1) rs1) (getReg (Regs s1) rs2)))
+                                    s1)))) s2) (= tt tt)))
+((Srl rd rs1 rs2) (and (=
+                        (withPc (NextPc s1)
+                           (withNextPc (bvadd (NextPc s1) ((_ int2bv 32) 4))
+                              (withDeps
+                                 (setDeps (Deps s1) rd (union (getDeps (Deps s1) rs1) (getDeps (Deps s1) rs2)))
+                                 (withRegs
+                                    (setReg (Regs s1) rd
+                                       (bvlshr (getReg (Regs s1) rs1)
+                                        ((_ int2bv 32) (mod ((_ bv2nat 32) (getReg (Regs s1) rs2)) 32)))) s1))))
+                        s2) (= tt tt)))
+((Sra rd rs1 rs2) (and (=
+                        (withPc (NextPc s1)
+                           (withNextPc (bvadd (NextPc s1) ((_ int2bv 32) 4))
+                              (withDeps
+                                 (setDeps (Deps s1) rd (union (getDeps (Deps s1) rs1) (getDeps (Deps s1) rs2)))
+                                 (withRegs
+                                    (setReg (Regs s1) rd
+                                       (bvashr (getReg (Regs s1) rs1)
+                                        ((_ int2bv 32) (mod ((_ bv2nat 32) (getReg (Regs s1) rs2)) 32)))) s1))))
+                        s2) (= tt tt)))
+((Or rd rs1 rs2) (and (=
+                       (withPc (NextPc s1)
+                          (withNextPc (bvadd (NextPc s1) ((_ int2bv 32) 4))
+                             (withDeps
+                                (setDeps (Deps s1) rd (union (getDeps (Deps s1) rs1) (getDeps (Deps s1) rs2)))
+                                (withRegs
+                                   (setReg (Regs s1) rd (bvor (getReg (Regs s1) rs1) (getReg (Regs s1) rs2)))
+                                   s1)))) s2) (= tt tt)))
+((And rd rs1 rs2) (and (=
+                        (withPc (NextPc s1)
+                           (withNextPc (bvadd (NextPc s1) ((_ int2bv 32) 4))
+                              (withDeps
+                                 (setDeps (Deps s1) rd (union (getDeps (Deps s1) rs1) (getDeps (Deps s1) rs2)))
+                                 (withRegs
+                                    (setReg (Regs s1) rd (bvand (getReg (Regs s1) rs1) (getReg (Regs s1) rs2)))
+                                    s1)))) s2) (= tt tt)))
+((Lui rd imm20) (and (=
+                      (withPc (NextPc s1)
+                         (withNextPc (bvadd (NextPc s1) ((_ int2bv 32) 4))
+                            (withDeps (Deps s1) (withRegs (setReg (Regs s1) rd ((_ int2bv 32) imm20)) s1))))
+                      s2) (= tt tt)))
+((Beq rs1 rs2 sbimm12) (ite (= (getReg (Regs s1) rs1) (getReg (Regs s1) rs2))
+                        (ite (not (= (bvurem (bvadd (Pc s1) ((_ int2bv 32) sbimm12)) ((_ int2bv 32) 4))
+                                   ((_ int2bv 32) 0)))
+                         (and (= (select (Lab G) (CurrentEvent s1)) ErrorLabel) (= s1 s2))
+                         (and (=
+                               (withPc (bvadd (Pc s1) ((_ int2bv 32) sbimm12))
+                                  (withNextPc
+                                     (bvadd (bvadd (Pc s1) ((_ int2bv 32) sbimm12)) ((_ int2bv 32) 4))
+                                     (withDeps
+                                        (setDeps (Deps s1) minusone
+                                           (union (getDeps (Deps s1) minusone)
+                                              (union (getDeps (Deps s1) rs1) (getDeps (Deps s1) rs2))))
+                                        (withNextPc (bvadd (Pc s1) ((_ int2bv 32) sbimm12)) s1)))) s2)
+                          (= tt tt)))
+                        (and (=
+                              (withPc (NextPc s1)
+                                 (withNextPc (bvadd (NextPc s1) ((_ int2bv 32) 4))
+                                    (withDeps
+                                       (setDeps (Deps s1) minusone
+                                          (union (getDeps (Deps s1) minusone)
+                                             (union (getDeps (Deps s1) rs1) (getDeps (Deps s1) rs2)))) s1)))
+                              s2) (= tt tt))))
+((Bne rs1 rs2 sbimm12) (ite (not (= (getReg (Regs s1) rs1) (getReg (Regs s1) rs2)))
+                        (ite (not (= (bvurem (bvadd (Pc s1) ((_ int2bv 32) sbimm12)) ((_ int2bv 32) 4))
+                                   ((_ int2bv 32) 0)))
+                         (and (= (select (Lab G) (CurrentEvent s1)) ErrorLabel) (= s1 s2))
+                         (and (=
+                               (withPc (bvadd (Pc s1) ((_ int2bv 32) sbimm12))
+                                  (withNextPc
+                                     (bvadd (bvadd (Pc s1) ((_ int2bv 32) sbimm12)) ((_ int2bv 32) 4))
+                                     (withDeps
+                                        (setDeps (Deps s1) minusone
+                                           (union (getDeps (Deps s1) minusone)
+                                              (union (getDeps (Deps s1) rs1) (getDeps (Deps s1) rs2))))
+                                        (withNextPc (bvadd (Pc s1) ((_ int2bv 32) sbimm12)) s1)))) s2)
+                          (= tt tt)))
+                        (and (=
+                              (withPc (NextPc s1)
+                                 (withNextPc (bvadd (NextPc s1) ((_ int2bv 32) 4))
+                                    (withDeps
+                                       (setDeps (Deps s1) minusone
+                                          (union (getDeps (Deps s1) minusone)
+                                             (union (getDeps (Deps s1) rs1) (getDeps (Deps s1) rs2)))) s1)))
+                              s2) (= tt tt))))
+((Blt rs1 rs2 sbimm12) (ite (bvslt (getReg (Regs s1) rs1) (getReg (Regs s1) rs2))
+                        (ite (not (= (bvurem (bvadd (Pc s1) ((_ int2bv 32) sbimm12)) ((_ int2bv 32) 4))
+                                   ((_ int2bv 32) 0)))
+                         (and (= (select (Lab G) (CurrentEvent s1)) ErrorLabel) (= s1 s2))
+                         (and (=
+                               (withPc (bvadd (Pc s1) ((_ int2bv 32) sbimm12))
+                                  (withNextPc
+                                     (bvadd (bvadd (Pc s1) ((_ int2bv 32) sbimm12)) ((_ int2bv 32) 4))
+                                     (withDeps
+                                        (setDeps (Deps s1) minusone
+                                           (union (getDeps (Deps s1) minusone)
+                                              (union (getDeps (Deps s1) rs1) (getDeps (Deps s1) rs2))))
+                                        (withNextPc (bvadd (Pc s1) ((_ int2bv 32) sbimm12)) s1)))) s2)
+                          (= tt tt)))
+                        (and (=
+                              (withPc (NextPc s1)
+                                 (withNextPc (bvadd (NextPc s1) ((_ int2bv 32) 4))
+                                    (withDeps
+                                       (setDeps (Deps s1) minusone
+                                          (union (getDeps (Deps s1) minusone)
+                                             (union (getDeps (Deps s1) rs1) (getDeps (Deps s1) rs2)))) s1)))
+                              s2) (= tt tt))))
+((Bge rs1 rs2 sbimm12) (ite (not (bvslt (getReg (Regs s1) rs1) (getReg (Regs s1) rs2)))
+                        (ite (not (= (bvurem (bvadd (Pc s1) ((_ int2bv 32) sbimm12)) ((_ int2bv 32) 4))
+                                   ((_ int2bv 32) 0)))
+                         (and (= (select (Lab G) (CurrentEvent s1)) ErrorLabel) (= s1 s2))
+                         (and (=
+                               (withPc (bvadd (Pc s1) ((_ int2bv 32) sbimm12))
+                                  (withNextPc
+                                     (bvadd (bvadd (Pc s1) ((_ int2bv 32) sbimm12)) ((_ int2bv 32) 4))
+                                     (withDeps
+                                        (setDeps (Deps s1) minusone
+                                           (union (getDeps (Deps s1) minusone)
+                                              (union (getDeps (Deps s1) rs1) (getDeps (Deps s1) rs2))))
+                                        (withNextPc (bvadd (Pc s1) ((_ int2bv 32) sbimm12)) s1)))) s2)
+                          (= tt tt)))
+                        (and (=
+                              (withPc (NextPc s1)
+                                 (withNextPc (bvadd (NextPc s1) ((_ int2bv 32) 4))
+                                    (withDeps
+                                       (setDeps (Deps s1) minusone
+                                          (union (getDeps (Deps s1) minusone)
+                                             (union (getDeps (Deps s1) rs1) (getDeps (Deps s1) rs2)))) s1)))
+                              s2) (= tt tt))))
+((Bltu rs1 rs2 sbimm12) (ite (bvult (getReg (Regs s1) rs1) (getReg (Regs s1) rs2))
+                         (ite (not (= (bvurem (bvadd (Pc s1) ((_ int2bv 32) sbimm12)) ((_ int2bv 32) 4))
+                                    ((_ int2bv 32) 0)))
+                          (and (= (select (Lab G) (CurrentEvent s1)) ErrorLabel) (= s1 s2))
+                          (and (=
+                                (withPc (bvadd (Pc s1) ((_ int2bv 32) sbimm12))
+                                   (withNextPc
+                                      (bvadd (bvadd (Pc s1) ((_ int2bv 32) sbimm12)) ((_ int2bv 32) 4))
+                                      (withDeps
+                                         (setDeps (Deps s1) minusone
+                                            (union (getDeps (Deps s1) minusone)
+                                               (union (getDeps (Deps s1) rs1) (getDeps (Deps s1) rs2))))
+                                         (withNextPc (bvadd (Pc s1) ((_ int2bv 32) sbimm12)) s1)))) s2)
+                           (= tt tt)))
+                         (and (=
+                               (withPc (NextPc s1)
+                                  (withNextPc (bvadd (NextPc s1) ((_ int2bv 32) 4))
+                                     (withDeps
+                                        (setDeps (Deps s1) minusone
+                                           (union (getDeps (Deps s1) minusone)
+                                              (union (getDeps (Deps s1) rs1) (getDeps (Deps s1) rs2)))) s1)))
+                               s2) (= tt tt))))
+((Bgeu rs1 rs2 sbimm12) (ite (not (bvult (getReg (Regs s1) rs1) (getReg (Regs s1) rs2)))
+                         (ite (not (= (bvurem (bvadd (Pc s1) ((_ int2bv 32) sbimm12)) ((_ int2bv 32) 4))
+                                    ((_ int2bv 32) 0)))
+                          (and (= (select (Lab G) (CurrentEvent s1)) ErrorLabel) (= s1 s2))
+                          (and (=
+                                (withPc (bvadd (Pc s1) ((_ int2bv 32) sbimm12))
+                                   (withNextPc
+                                      (bvadd (bvadd (Pc s1) ((_ int2bv 32) sbimm12)) ((_ int2bv 32) 4))
+                                      (withDeps
+                                         (setDeps (Deps s1) minusone
+                                            (union (getDeps (Deps s1) minusone)
+                                               (union (getDeps (Deps s1) rs1) (getDeps (Deps s1) rs2))))
+                                         (withNextPc (bvadd (Pc s1) ((_ int2bv 32) sbimm12)) s1)))) s2)
+                           (= tt tt)))
+                         (and (=
+                               (withPc (NextPc s1)
+                                  (withNextPc (bvadd (NextPc s1) ((_ int2bv 32) 4))
+                                     (withDeps
+                                        (setDeps (Deps s1) minusone
+                                           (union (getDeps (Deps s1) minusone)
+                                              (union (getDeps (Deps s1) rs1) (getDeps (Deps s1) rs2)))) s1)))
+                               s2) (= tt tt))))
+((Jalr rd rs1 oimm12) (ite (not (=
+                                 (bvurem (bvand (bvadd (getReg (Regs s1) rs1) ((_ int2bv 32) oimm12))
+                                          (bvxor ((_ int2bv 32) 1) ((_ int2bv 32) 4294967295)))
+                                  ((_ int2bv 32) 4)) ((_ int2bv 32) 0)))
+                       (and (= (select (Lab G) (CurrentEvent s1)) ErrorLabel) (= s1 s2))
+                       (and (=
+                             (withPc
+                                (bvand (bvadd (getReg (Regs s1) rs1) ((_ int2bv 32) oimm12))
+                                 (bvxor ((_ int2bv 32) 1) ((_ int2bv 32) 4294967295)))
+                                (withNextPc
+                                   (bvadd (bvand (bvadd (getReg (Regs s1) rs1) ((_ int2bv 32) oimm12))
+                                           (bvxor ((_ int2bv 32) 1) ((_ int2bv 32) 4294967295)))
+                                    ((_ int2bv 32) 4))
+                                   (withDeps
+                                      (setDeps (setDeps (Deps s1) rd (getDeps (Deps s1) minusone)) minusone
+                                         (union (getDeps (Deps s1) minusone) (getDeps (Deps s1) rs1)))
+                                      (withNextPc
+                                         (bvand (bvadd (getReg (Regs s1) rs1) ((_ int2bv 32) oimm12))
+                                          (bvxor ((_ int2bv 32) 1) ((_ int2bv 32) 4294967295)))
+                                         (withRegs (setReg (Regs s1) rd (bvadd (Pc s1) ((_ int2bv 32) 4))) s1)))))
+                             s2) (= tt tt))))
+((Jal rd jimm20) (ite (not (= (bvurem (bvadd (Pc s1) ((_ int2bv 32) jimm20)) ((_ int2bv 32) 4))
+                            ((_ int2bv 32) 0)))
+                  (and (= (select (Lab G) (CurrentEvent s1)) ErrorLabel) (= s1 s2))
+                  (and (=
+                        (withPc (bvadd (Pc s1) ((_ int2bv 32) jimm20))
+                           (withNextPc (bvadd (bvadd (Pc s1) ((_ int2bv 32) jimm20)) ((_ int2bv 32) 4))
+                              (withDeps (setDeps (Deps s1) rd (getDeps (Deps s1) minusone))
+                                 (withNextPc (bvadd (Pc s1) ((_ int2bv 32) jimm20))
+                                    (withRegs (setReg (Regs s1) rd (bvadd (Pc s1) ((_ int2bv 32) 4))) s1)))))
+                        s2) (= tt tt))))
+((InvalidI) (and (=
+                  (withPc (NextPc s1)
+                     (withNextPc (bvadd (NextPc s1) ((_ int2bv 32) 4)) (withDeps (Deps s1) s1))) s2)
+             (= tt tt)))))
+)
+
+(declare-const G Graph)
+(declare-const s1 ThreadState)
+(declare-const s2 ThreadState)
+(assert (run1 G s1 s2))
 (check-sat)
 (get-model)
